<?xml version="1.0" encoding="UTF-8"?>
<rdf:RDF
   xmlns:cc="http://creativecommons.org/ns#"
   xmlns:dc="http://purl.org/dc/elements/1.1/"
   xmlns:foaf="http://xmlns.com/foaf/0.1/"
   xmlns:owl="http://www.w3.org/2002/07/owl#"
   xmlns:rdf="http://www.w3.org/1999/02/22-rdf-syntax-ns#"
   xmlns:rdfs="http://www.w3.org/2000/01/rdf-schema#"
>
  <rdf:Description rdf:about="http://linkedopendatang.com/schemas/election#hasVotes">
    <rdfs:comment>This property associates an instance of Poll or PollingBooth with total votes casted</rdfs:comment>
    <rdfs:range rdf:resource="http://www.w3.org/2001/XMLSchema#integer"/>
    <rdfs:isDefinedBy rdf:resource="http://linkedopendatang.com/schemas/election/"/>
    <rdfs:domain rdf:resource="http://linkedopendatang.com/schemas/election#PollingBooth"/>
    <rdf:type rdf:resource="http://www.w3.org/2002/07/owl#DatatypeProperty"/>
    <rdfs:domain rdf:resource="http://linkedopendatang.com/schemas/election#Poll"/>
    <rdfs:label>hasVotes</rdfs:label>
  </rdf:Description>
  <rdf:Description rdf:about="http://linkedopendatang.com/schemas/election#isOfPoliticalParty">
    <rdfs:isDefinedBy rdf:resource="http://linkedopendatang.com/schemas/election/"/>
    <rdfs:domain rdf:resource="http://linkedopendatang.com/schemas/election#Candidate"/>
    <rdfs:comment>This property associates an instance of Candidate with an instance of PoliticalParty</rdfs:comment>
    <rdf:type rdf:resource="http://www.w3.org/2002/07/owl#DatatypeProperty"/>
    <rdfs:range rdf:resource="http://linkedopendatang.com/schemas/election#PoliticalParty"/>
    <rdfs:label>isOfPoliticalParty</rdfs:label>
  </rdf:Description>
  <rdf:Description rdf:about="http://linkedopendatang.com/schemas/election#Election">
    <rdf:type rdf:resource="http://www.w3.org/2002/07/owl#Class"/>
    <rdfs:isDefinedBy rdf:resource="http://linkedopendatang.com/schemas/election/"/>
    <rdfs:comment>A class representing a set of polls</rdfs:comment>
    <rdfs:subClassOf rdf:resource="http://linkedopendatang.com/schemas/election#Object"/>
    <rdfs:label>Election</rdfs:label>
    <rdfs:subClassOf rdf:resource="http://schema.org/Event"/>
  </rdf:Description>
  <rdf:Description rdf:about="http://linkedopendatang.com/schemas/election#hasTotalBallots">
    <rdfs:range rdf:resource="http://www.w3.org/2001/XMLSchema#integer"/>
    <rdf:type rdf:resource="http://www.w3.org/2002/07/owl#DatatypeProperty"/>
    <rdfs:domain rdf:resource="http://linkedopendatang.com/schemas/election#Poll"/>
    <rdfs:label>hasTotalBallots</rdfs:label>
    <rdfs:comment>This property associates an instance of Poll or PollingBooth with the total number of casted ballots</rdfs:comment>
    <rdfs:domain rdf:resource="http://linkedopendatang.com/schemas/election#PollingBooth"/>
    <rdfs:isDefinedBy rdf:resource="http://linkedopendatang.com/schemas/election/"/>
  </rdf:Description>
  <rdf:Description rdf:about="http://linkedopendatang.com/schemas/election#hasValidBallots">
    <rdfs:isDefinedBy rdf:resource="http://linkedopendatang.com/schemas/election/"/>
    <rdfs:range rdf:resource="http://www.w3.org/2001/XMLSchema#integer"/>
    <rdfs:comment>This property associates an instance of Poll or PoollingBooth with the total number of valid ballots</rdfs:comment>
    <rdf:type rdf:resource="http://www.w3.org/2002/07/owl#DatatypeProperty"/>
    <rdfs:domain rdf:resource="http://linkedopendatang.com/schemas/election#Poll"/>
    <rdfs:domain rdf:resource="http://linkedopendatang.com/schemas/election#PollingBooth"/>
    <rdfs:label>hasValidBallots</rdfs:label>
  </rdf:Description>
  <rdf:Description rdf:about="http://linkedopendatang.com/schemas/election#Poll">
    <rdfs:subClassOf rdf:resource="http://linkedopendatang.com/schemas/election#Object"/>
    <rdfs:subClassOf rdf:resource="http://schema.org/Event"/>
    <rdf:type rdf:resource="http://www.w3.org/2002/07/owl#Class"/>
    <rdfs:isDefinedBy rdf:resource="http://linkedopendatang.com/schemas/election/"/>
    <rdfs:comment>A class representing a voting event to select a political leader</rdfs:comment>
    <rdfs:label>Poll</rdfs:label>
  </rdf:Description>
  <rdf:Description rdf:about="http://linkedopendatang.com/schemas/election#hasViolence">
    <rdfs:isDefinedBy rdf:resource="http://linkedopendatang.com/schemas/election/"/>
    <rdfs:label>hasViolence</rdfs:label>
    <rdfs:domain rdf:resource="http://linkedopendatang.com/schemas/election#PollingBooth"/>
    <rdfs:comment>This property associates an instance of Poll or PollingBooth with a violence status</rdfs:comment>
    <rdf:type rdf:resource="http://www.w3.org/2002/07/owl#DatatypeProperty"/>
    <rdfs:domain rdf:resource="http://linkedopendatang.com/schemas/election#Poll"/>
    <rdfs:range rdf:resource="http://www.w3.org/2001/XMLSchema#boolean"/>
  </rdf:Description>
  <rdf:Description rdf:about="http://linkedopendatang.com/schemas/election#isElected">
    <rdf:type rdf:resource="http://www.w3.org/2002/07/owl#DatatypeProperty"/>
    <rdfs:label>elected</rdfs:label>
    <rdfs:domain rdf:resource="http://linkedopendatang.com/schemas/election#Candidate"/>
    <rdfs:range rdf:resource="http://www.w3.org/2001/XMLSchema#boolean"/>
    <rdfs:isDefinedBy rdf:resource="http://linkedopendatang.com/schemas/election/"/>
    <rdfs:comment>This property associates an instance of Candidate with an elected status</rdfs:comment>
  </rdf:Description>
  <rdf:Description rdf:about="http://linkedopendatang.com/schemas/election#hasURL">
    <rdfs:isDefinedBy rdf:resource="http://linkedopendatang.com/schemas/election/"/>
    <rdfs:range rdf:resource="http://www.w3.org/2001/XMLSchema#anyURI"/>
    <rdfs:comment>This property associates an instance of Candidate with a resource that has more information on Candidate</rdfs:comment>
    <rdfs:domain rdf:resource="http://linkedopendatang.com/schemas/election#Candidate"/>
    <rdfs:label>hasURL</rdfs:label>
    <rdf:type rdf:resource="http://www.w3.org/2002/07/owl#DatatypeProperty"/>
  </rdf:Description>
  <rdf:Description rdf:about="http://linkedopendatang.com/schemas/election#PollingBooth">
    <rdfs:label>PollingBooth</rdfs:label>
    <rdfs:comment>A booth where a voting event to select a political leader is held</rdfs:comment>
    <rdf:type rdf:resource="http://www.w3.org/2002/07/owl#Class"/>
    <rdfs:subClassOf rdf:resource="http://linkedopendatang.com/schemas/election#Poll"/>
    <rdfs:isDefinedBy rdf:resource="http://linkedopendatang.com/schemas/election/"/>
  </rdf:Description>
  <rdf:Description rdf:about="http://linkedopendatang.com/schemas/election#isCandidate">
    <rdfs:label>isCandidate</rdfs:label>
    <rdfs:isDefinedBy rdf:resource="http://linkedopendatang.com/schemas/election/"/>
    <rdfs:domain rdf:resource="http://linkedopendatang.com/schemas/election#Poll"/>
    <rdf:type rdf:resource="http://www.w3.org/2002/07/owl#DatatypeProperty"/>
    <rdfs:comment>This property associates an instance of Poll with an instance of Candidate</rdfs:comment>
    <rdfs:range rdf:resource="http://linkedopendatang.com/schemas/election#Candidate"/>
  </rdf:Description>
  <rdf:Description rdf:about="http://linkedopendatang.com/schemas/election#hasGeoLat">
    <rdfs:domain rdf:resource="http://linkedopendatang.com/schemas/election#PollingBooth"/>
    <rdf:type rdf:resource="http://www.w3.org/2002/07/owl#DatatypeProperty"/>
    <rdfs:range rdf:resource="http://www.w3.org/2003/01/geo/wgs84_pos#lat"/>
    <rdfs:label>hasGeoLatitude</rdfs:label>
    <rdfs:isDefinedBy rdf:resource="http://linkedopendatang.com/schemas/election/"/>
    <rdfs:comment>This property associates an instance of PollingBooth with an instance of geo:lat</rdfs:comment>
  </rdf:Description>
  <rdf:Description rdf:about="http://linkedopendatang.com/schemas/election/">
    <rdfs:comment rdf:datatype="http://www.w3.org/2001/XMLSchema#string">This is a turtle document that uses Linked Data oriented content to describe an Ontology for Elections</rdfs:comment>
    <owl:versionInfo rdf:datatype="http://www.w3.org/2001/XMLSchema#string">0.1.0</owl:versionInfo>
    <rdfs:label>An Ontology for Linked Open Election Data</rdfs:label>
    <rdf:type rdf:resource="http://www.w3.org/2002/07/owl#Ontology"/>
    <dc:date rdf:datatype="http://www.w3.org/2001/XMLSchema#date">2014-11-01</dc:date>
    <foaf:maker rdf:resource="http://id.myopenlink.net/dataspace/person/emekaokoye#this"/>
    <cc:license rdf:resource="http://creativecommons.org/licenses/by-sa/3.0/"/>
  </rdf:Description>
  <rdf:Description rdf:about="http://linkedopendatang.com/schemas/election#hasConstituency">
    <rdfs:range rdf:resource="http://schema.org/Place"/>
    <rdfs:domain rdf:resource="http://linkedopendatang.com/schemas/election#Candidate"/>
    <rdfs:domain rdf:resource="http://linkedopendatang.com/schemas/election#Poll"/>
    <rdf:type rdf:resource="http://www.w3.org/2002/07/owl#DatatypeProperty"/>
    <rdfs:label>hasConstituency</rdfs:label>
    <rdfs:isDefinedBy rdf:resource="http://linkedopendatang.com/schemas/election/"/>
    <rdfs:comment>This property associates an instance of Poll or Candidate with an instance of Place</rdfs:comment>
  </rdf:Description>
  <rdf:Description rdf:about="http://linkedopendatang.com/schemas/election#hasElectionDate">
    <rdfs:domain rdf:resource="http://linkedopendatang.com/schemas/election#Poll"/>
    <rdfs:isDefinedBy rdf:resource="http://linkedopendatang.com/schemas/election/"/>
    <rdf:type rdf:resource="http://www.w3.org/2002/07/owl#DatatypeProperty"/>
    <rdfs:label>hasElectionDate</rdfs:label>
    <rdfs:comment>This property associates an instance of Poll with a date</rdfs:comment>
    <rdfs:range rdf:resource="http://www.w3.org/2001/XMLSchema#date"/>
  </rdf:Description>
  <rdf:Description rdf:about="http://linkedopendatang.com/schemas/election#hasRegisteredVoters">
    <rdfs:range rdf:resource="http://www.w3.org/2001/XMLSchema#integer"/>
    <rdfs:label>hasRegisteredVoters</rdfs:label>
    <rdfs:isDefinedBy rdf:resource="http://linkedopendatang.com/schemas/election/"/>
    <rdfs:comment>This property associates an instance of Poll with the total number of registered voters</rdfs:comment>
    <rdf:type rdf:resource="http://www.w3.org/2002/07/owl#DatatypeProperty"/>
    <rdfs:domain rdf:resource="http://linkedopendatang.com/schemas/election#Poll"/>
  </rdf:Description>
  <rdf:Description rdf:about="http://linkedopendatang.com/schemas/election#PoliticalParty">
    <rdfs:comment>A class representing a Political Party</rdfs:comment>
    <rdf:type rdf:resource="http://www.w3.org/2002/07/owl#Class"/>
    <rdfs:isDefinedBy rdf:resource="http://linkedopendatang.com/schemas/election/"/>
    <rdfs:subClassOf rdf:resource="http://schema.org/Organization"/>
    <rdfs:label>PoliticalParty</rdfs:label>
    <rdfs:subClassOf rdf:resource="http://xmlns.com/foaf/0.1/Organization"/>
  </rdf:Description>
  <rdf:Description rdf:about="http://linkedopendatang.com/schemas/election#Object">
    <rdf:type rdf:resource="http://www.w3.org/2002/07/owl#Class"/>
    <rdfs:label>ElectionObject</rdfs:label>
    <rdfs:isDefinedBy rdf:resource="http://linkedopendatang.com/schemas/election/"/>
    <rdfs:comment>A base class representing all Election objects</rdfs:comment>
  </rdf:Description>
  <rdf:Description rdf:about="http://linkedopendatang.com/schemas/election#hasElectoralFraud">
    <rdfs:domain rdf:resource="http://linkedopendatang.com/schemas/election#PollingBooth"/>
    <rdfs:isDefinedBy rdf:resource="http://linkedopendatang.com/schemas/election/"/>
    <rdfs:domain rdf:resource="http://linkedopendatang.com/schemas/election#Poll"/>
    <rdfs:label>hasElectoralFraud</rdfs:label>
    <rdfs:range rdf:resource="http://www.w3.org/2001/XMLSchema#boolean"/>
    <rdfs:comment>This property associates an instance of Poll or PollingBooth with electoral fraud status</rdfs:comment>
    <rdf:type rdf:resource="http://www.w3.org/2002/07/owl#DatatypeProperty"/>
  </rdf:Description>
  <rdf:Description rdf:about="http://linkedopendatang.com/schemas/election#Candidate">
    <rdfs:subClassOf rdf:resource="http://xmlns.com/foaf/0.1/Person"/>
    <rdfs:label>Candidate</rdfs:label>
    <rdfs:subClassOf rdf:resource="http://schema.org/Person"/>
    <rdf:type rdf:resource="http://www.w3.org/2002/07/owl#Class"/>
    <rdfs:comment>A class representing a Person seeking an elective office</rdfs:comment>
    <rdfs:isDefinedBy rdf:resource="http://linkedopendatang.com/schemas/election/"/>
  </rdf:Description>
  <rdf:Description rdf:about="http://linkedopendatang.com/schemas/election#hasInvalidBallots">
    <rdfs:range rdf:resource="http://www.w3.org/2001/XMLSchema#integer"/>
    <rdfs:isDefinedBy rdf:resource="http://linkedopendatang.com/schemas/election/"/>
    <rdfs:domain rdf:resource="http://linkedopendatang.com/schemas/election#PollingBooth"/>
    <rdfs:label>hasInvalidBallots</rdfs:label>
    <rdfs:comment>This property associates an instance of Poll or PollingBooth with the total number of invalid ballots</rdfs:comment>
    <rdfs:domain rdf:resource="http://linkedopendatang.com/schemas/election#Poll"/>
    <rdf:type rdf:resource="http://www.w3.org/2002/07/owl#DatatypeProperty"/>
  </rdf:Description>
  <rdf:Description rdf:about="http://linkedopendatang.com/schemas/election#isWinner">
    <rdfs:label>isWinner</rdfs:label>
    <rdfs:range rdf:resource="http://www.w3.org/2001/XMLSchema#boolean"/>
    <rdf:type rdf:resource="http://www.w3.org/2002/07/owl#DatatypeProperty"/>
    <rdfs:domain rdf:resource="http://linkedopendatang.com/schemas/election#Candidate"/>
    <rdfs:comment>This property associates an instance of Candidate with a winner status</rdfs:comment>
    <rdfs:isDefinedBy rdf:resource="http://linkedopendatang.com/schemas/election/"/>
  </rdf:Description>
  <rdf:Description rdf:about="http://linkedopendatang.com/schemas/election#hasGeoLong">
    <rdfs:comment>This property associates an instance of PollingBooth with an instance of geo:long</rdfs:comment>
    <rdfs:range rdf:resource="http://www.w3.org/2003/01/geo/wgs84_pos#long"/>
    <rdfs:isDefinedBy rdf:resource="http://linkedopendatang.com/schemas/election/"/>
    <rdf:type rdf:resource="http://www.w3.org/2002/07/owl#DatatypeProperty"/>
    <rdfs:domain rdf:resource="http://linkedopendatang.com/schemas/election#PollingBooth"/>
    <rdfs:label>hasGeoLongtitude</rdfs:label>
  </rdf:Description>
  <rdf:Description rdf:about="http://linkedopendatang.com/schemas/election#image">
    <rdfs:isDefinedBy rdf:resource="http://linkedopendatang.com/schemas/election/"/>
    <rdfs:domain rdf:resource="http://linkedopendatang.com/schemas/election#Candidate"/>
    <rdfs:label>image</rdfs:label>
    <rdfs:range rdf:resource="http://xmlns.com/foaf/0.1/depiction"/>
    <rdfs:comment>This property associates an instance of Candidate with an instance of foaf:depiction</rdfs:comment>
    <rdf:type rdf:resource="http://www.w3.org/2002/07/owl#DatatypeProperty"/>
  </rdf:Description>
  <rdf:Description rdf:about="http://linkedopendatang.com/schemas/election#hasName">
    <rdfs:isDefinedBy rdf:resource="http://linkedopendatang.com/schemas/election/"/>
    <rdfs:comment>This property associates an instance of Candidate with names</rdfs:comment>
    <rdfs:label>hasName</rdfs:label>
    <rdf:type rdf:resource="http://www.w3.org/2002/07/owl#DatatypeProperty"/>
    <rdfs:domain rdf:resource="http://linkedopendatang.com/schemas/election#Candidate"/>
    <rdfs:range rdf:resource="http://schema.org/Person"/>
    <rdfs:range rdf:resource="http://xmlns.com/foaf/0.1/Person"/>
  </rdf:Description>
  <rdf:Description rdf:about="http://linkedopendatang.com/schemas/election#hasAccreditedVoters">
    <rdfs:isDefinedBy rdf:resource="http://linkedopendatang.com/schemas/election/"/>
    <rdfs:range rdf:resource="http://www.w3.org/2001/XMLSchema#integer"/>
    <rdfs:domain rdf:resource="http://linkedopendatang.com/schemas/election#Poll"/>
    <rdf:type rdf:resource="http://www.w3.org/2002/07/owl#DatatypeProperty"/>
    <rdfs:label>hasAccreditedVoters</rdfs:label>
    <rdfs:comment>This property associates an instance of Poll with the total number of accredited voters</rdfs:comment>
  </rdf:Description>
  <rdf:Description rdf:about="http://id.myopenlink.net/dataspace/person/emekaokoye#this">
    <rdf:type rdf:resource="http://xmlns.com/foaf/0.1/Person"/>
    <foaf:name>Emeka Okoye</foaf:name>
  </rdf:Description>
</rdf:RDF>

