
#
# An Ontology for Linked Open Election Data 
#


@prefix cc: <http://creativecommons.org/ns#> .
@prefix dc: <http://purl.org/dc/elements/1.1/> .
@prefix dcterms: <http://purl.org/dc/terms/> .
@prefix foaf: <http://xmlns.com/foaf/0.1/> .
@prefix owl: <http://www.w3.org/2002/07/owl#> .
@prefix rdf: <http://www.w3.org/1999/02/22-rdf-syntax-ns#> .
@prefix rdfs: <http://www.w3.org/2000/01/rdf-schema#> .
@prefix xsd: <http://www.w3.org/2001/XMLSchema#> .
@prefix geo: <http://www.w3.org/2003/01/geo/wgs84_pos#> .
@prefix schema: <http://schema.org/> .


@prefix election: <http://linkedopendatang.com/schemas/election#> .

<http://linkedopendatang.com/schemas/election/>
	a owl:Ontology ;
	rdfs:label "An Ontology for Linked Open Election Data" ;
	cc:license <http://creativecommons.org/licenses/by-sa/3.0/> ;
	dc:date "2014-11-01"^^xsd:date ;
	foaf:maker <http://id.myopenlink.net/dataspace/person/emekaokoye#this> ;
	rdfs:comment """This is a turtle document that uses Linked Data oriented content to describe an Ontology for Elections"""^^xsd:string ;
   owl:versionInfo "0.1.0"^^xsd:string .

<http://id.myopenlink.net/dataspace/person/emekaokoye#this> a foaf:Person ;
  foaf:name "Emeka Okoye" .
  
#
# Classes 
#


election:Object
    a owl:Class;
    rdfs:isDefinedBy <http://linkedopendatang.com/schemas/election/> ;
    rdfs:label "ElectionObject" ;
    rdfs:comment "A base class representing all Election objects" .
	
	
election:PoliticalParty
    a owl:Class;
    rdfs:isDefinedBy <http://linkedopendatang.com/schemas/election/> ;
    rdfs:subClassOf foaf:Organization, schema:Organization ;
    rdfs:label "PoliticalParty" ;
    rdfs:comment "A class representing a Political Party" .
	
	
election:Candidate
    a owl:Class;
    rdfs:isDefinedBy <http://linkedopendatang.com/schemas/election/> ;
    rdfs:subClassOf foaf:Person,schema:Person ;
    rdfs:label "Candidate" ;
    rdfs:comment "A class representing a Person seeking an elective office" .
	
	
election:Poll
    a owl:Class;
    rdfs:isDefinedBy <http://linkedopendatang.com/schemas/election/> ;
    rdfs:subClassOf election:Object ;
    rdfs:subClassOf schema:Event ;
    rdfs:label "Poll" ;
    rdfs:comment "A class representing a voting event to select a political leader" .
	
	
election:PollingBooth
    a owl:Class;
    rdfs:isDefinedBy <http://linkedopendatang.com/schemas/election/> ;
    rdfs:subClassOf election:Poll ;
    rdfs:label "PollingBooth" ;
    rdfs:comment "A booth where a voting event to select a political leader is held" .
	
	
election:Election
    a owl:Class;
    rdfs:isDefinedBy <http://linkedopendatang.com/schemas/election/> ;
    rdfs:subClassOf election:Object ;
    rdfs:subClassOf schema:Event ;
    rdfs:label "Election" ;
    rdfs:comment "A class representing a set of polls" .
	
	
	
	
#
# Properties 
#

	
election:hasConstituency
    a owl:DatatypeProperty ;
    rdfs:isDefinedBy <http://linkedopendatang.com/schemas/election/> ;
    rdfs:label "hasConstituency" ;
    rdfs:comment "This property associates an instance of Poll or Candidate with an instance of Place" ;
    rdfs:domain election:Poll,election:Candidate ;
    rdfs:range schema:Place .
	
	
election:isCandidate
    a owl:DatatypeProperty ;
    rdfs:isDefinedBy <http://linkedopendatang.com/schemas/election/> ;
    rdfs:label "isCandidate" ;
    rdfs:comment "This property associates an instance of Poll with an instance of Candidate" ;
    rdfs:domain election:Poll ;
    rdfs:range election:Candidate .
	
	
election:hasVotes
    a owl:DatatypeProperty ;
    rdfs:isDefinedBy <http://linkedopendatang.com/schemas/election/> ;
    rdfs:label "hasVotes" ;
    rdfs:comment "This property associates an instance of Poll or PollingBooth with total votes casted" ;
    rdfs:domain election:Poll,election:PollingBooth ;
    rdfs:range xsd:integer .
	
	
election:hasRegisteredVoters
    a owl:DatatypeProperty ;
    rdfs:isDefinedBy <http://linkedopendatang.com/schemas/election/> ;
    rdfs:label "hasRegisteredVoters" ;
    rdfs:comment "This property associates an instance of Poll with the total number of registered voters" ;
    rdfs:domain election:Poll ;
    rdfs:range xsd:integer .
	
	
election:hasAccreditedVoters
    a owl:DatatypeProperty ;
    rdfs:isDefinedBy <http://linkedopendatang.com/schemas/election/> ;
    rdfs:label "hasAccreditedVoters" ;
    rdfs:comment "This property associates an instance of Poll with the total number of accredited voters" ;
    rdfs:domain election:Poll ;
    rdfs:range xsd:integer .
	
	
election:hasTotalBallots
    a owl:DatatypeProperty ;
    rdfs:isDefinedBy <http://linkedopendatang.com/schemas/election/> ;
    rdfs:label "hasTotalBallots" ;
    rdfs:comment "This property associates an instance of Poll or PollingBooth with the total number of casted ballots" ;
    rdfs:domain election:Poll,election:PollingBooth ;
    rdfs:range xsd:integer .
	
	
election:hasInvalidBallots
    a owl:DatatypeProperty ;
    rdfs:isDefinedBy <http://linkedopendatang.com/schemas/election/> ;
    rdfs:label "hasInvalidBallots" ;
    rdfs:comment "This property associates an instance of Poll or PollingBooth with the total number of invalid ballots" ;
    rdfs:domain election:Poll,election:PollingBooth ;
    rdfs:range xsd:integer .
	
election:hasValidBallots
    a owl:DatatypeProperty ;
    rdfs:isDefinedBy <http://linkedopendatang.com/schemas/election/> ;
    rdfs:label "hasValidBallots" ;
    rdfs:comment "This property associates an instance of Poll or PoollingBooth with the total number of valid ballots" ;
    rdfs:domain election:Poll,election:PollingBooth ;
    rdfs:range xsd:integer .
	
election:isOfPoliticalParty
    a owl:DatatypeProperty ;
    rdfs:isDefinedBy <http://linkedopendatang.com/schemas/election/> ;
    rdfs:label "isOfPoliticalParty" ;
    rdfs:comment "This property associates an instance of Candidate with an instance of PoliticalParty" ;
    rdfs:domain election:Candidate ;
    rdfs:range election:PoliticalParty .
	
election:hasName
    a owl:DatatypeProperty ;
    rdfs:isDefinedBy <http://linkedopendatang.com/schemas/election/> ;
    rdfs:label "hasName" ;
    rdfs:comment "This property associates an instance of Candidate with names" ;
    rdfs:domain election:Candidate ;
    rdfs:range foaf:Person,schema:Person .
	
	
election:isElected
    a owl:DatatypeProperty ;
    rdfs:isDefinedBy <http://linkedopendatang.com/schemas/election/> ;
    rdfs:label "elected" ;
    rdfs:comment "This property associates an instance of Candidate with an elected status" ;
    rdfs:domain election:Candidate ;
    rdfs:range xsd:boolean .
	
	
election:isWinner
    a owl:DatatypeProperty ;
    rdfs:isDefinedBy <http://linkedopendatang.com/schemas/election/> ;
    rdfs:label "isWinner" ;
    rdfs:comment "This property associates an instance of Candidate with a winner status" ;
    rdfs:domain election:Candidate ;
    rdfs:range xsd:boolean .
	
	
election:hasViolence
    a owl:DatatypeProperty ;
    rdfs:isDefinedBy <http://linkedopendatang.com/schemas/election/> ;
    rdfs:label "hasViolence" ;
    rdfs:comment "This property associates an instance of Poll or PollingBooth with a violence status" ;
    rdfs:domain election:Poll,election:PollingBooth ;
    rdfs:range xsd:boolean .
	
	
election:hasElectoralFraud
    a owl:DatatypeProperty ;
    rdfs:isDefinedBy <http://linkedopendatang.com/schemas/election/> ;
    rdfs:label "hasElectoralFraud" ;
    rdfs:comment "This property associates an instance of Poll or PollingBooth with electoral fraud status" ;
    rdfs:domain election:Poll,election:PollingBooth ;
    rdfs:range xsd:boolean .
	
	
election:image
    a owl:DatatypeProperty ;
    rdfs:isDefinedBy <http://linkedopendatang.com/schemas/election/> ;
    rdfs:label "image" ;
    rdfs:comment "This property associates an instance of Candidate with an instance of foaf:depiction" ;
    rdfs:domain election:Candidate ;
    rdfs:range foaf:depiction .
	
	
election:hasURL
    a owl:DatatypeProperty ;
    rdfs:isDefinedBy <http://linkedopendatang.com/schemas/election/> ;
    rdfs:label "hasURL" ;
    rdfs:comment "This property associates an instance of Candidate with a resource that has more information on Candidate" ;
    rdfs:domain election:Candidate ;
    rdfs:range xsd:anyURI .
	
	
election:hasElectionDate
    a owl:DatatypeProperty ;
    rdfs:isDefinedBy <http://linkedopendatang.com/schemas/election/> ;
    rdfs:label "hasElectionDate" ;
    rdfs:comment "This property associates an instance of Poll with a date" ;
    rdfs:domain election:Poll ;
    rdfs:range xsd:date .
	
	
election:hasGeoLat
    a owl:DatatypeProperty ;
    rdfs:isDefinedBy <http://linkedopendatang.com/schemas/election/> ;
    rdfs:label "hasGeoLatitude" ;
    rdfs:comment "This property associates an instance of PollingBooth with an instance of geo:lat" ;
    rdfs:domain election:PollingBooth ;
    rdfs:range geo:lat .
	
	
election:hasGeoLong
    a owl:DatatypeProperty ;
    rdfs:isDefinedBy <http://linkedopendatang.com/schemas/election/> ;
    rdfs:label "hasGeoLongtitude" ;
    rdfs:comment "This property associates an instance of PollingBooth with an instance of geo:long" ;
    rdfs:domain election:PollingBooth ;
    rdfs:range geo:long .
	
	
#
# todo 
#
# from revoda @en-gb
#
# inec -> INEC official arrival status {y|n|l} -> {yes,no,late}
# mate -> Materials Availability status {y|n|l} -> {yes,no,late}
# vote -> voting & accreditation status {y|n|l} -> {yes,no,late}
# coll -> vote collation and count status {y|n|l} -> {yes,no,late}
# anno -> Result Annoucement status {y|n} -> {yes,no}

	
	
	
